complete revision: finally got rid of annoying L-predicate

src/HOL/IMP/Abs_Int1.thy
@@ -4,6 +4,20 @@ theory Abs_Int1
 imports Abs_State
 begin
 
+(* FIXME mv *)
+instantiation acom :: (type) vars
+begin
+
+definition "vars_acom = vars o strip"
+
+instance ..
+
+end
+
+lemma finite_Cvars: "finite(vars(C::'a acom))"
+by(simp add: vars_acom_def)
+
+
 lemma le_iff_le_annos_zip: "C1 \<le> C2 \<longleftrightarrow>
  (\<forall> (a1,a2) \<in> set(zip (annos C1) (annos C2)). a1 \<le> a2) \<and> strip C1 = strip C2"
 by(induct C1 C2 rule: less_eq_acom.induct) (auto simp: size_annos_same2)
@@ -12,27 +26,9 @@ lemma le_iff_le_annos: "C1 \<le> C2 \<longleftrightarrow>
   strip C1 = strip C2 \<and> (\<forall> i<size(annos C1). annos C1 ! i \<le> annos C2 ! i)"
 by(auto simp add: le_iff_le_annos_zip set_zip) (metis size_annos_same2)
 
-
-lemma mono_fun_L[simp]: "F \<in> L X \<Longrightarrow> F \<le> G \<Longrightarrow> x : X \<Longrightarrow> fun F x \<le> fun G x"
-by(simp add: mono_fun L_st_def)
-
-lemma bot_in_L[simp]: "bot c \<in> L(vars c)"
-by(simp add: L_acom_def bot_def)
-
-lemma L_acom_simps[simp]: "SKIP {P} \<in> L X \<longleftrightarrow> P \<in> L X"
-  "(x ::= e {P}) \<in> L X \<longleftrightarrow> x : X \<and> vars e \<subseteq> X \<and> P \<in> L X"
-  "(C1;C2) \<in> L X \<longleftrightarrow> C1 \<in> L X \<and> C2 \<in> L X"
-  "(IF b THEN {P1} C1 ELSE {P2} C2 {Q}) \<in> L X \<longleftrightarrow>
-   vars b \<subseteq> X \<and> C1 \<in> L X \<and> C2 \<in> L X \<and> P1 \<in> L X \<and> P2 \<in> L X \<and> Q \<in> L X"
-  "({I} WHILE b DO {P} C {Q}) \<in> L X \<longleftrightarrow>
-   I \<in> L X \<and> vars b \<subseteq> X \<and> P \<in> L X \<and> C \<in> L X \<and> Q \<in> L X"
-by(auto simp add: L_acom_def)
-
-lemma post_in_annos: "post C : set(annos C)"
+(* FIXME mv *)
+lemma post_in_annos: "post C \<in> set(annos C)"
 by(induction C) auto
-
-lemma post_in_L[simp]: "C \<in> L X \<Longrightarrow> post C \<in> L X"
-by(simp add: L_acom_def post_in_annos)
 
 
 subsection "Computable Abstract Interpretation"
@@ -47,30 +43,20 @@ fun aval' :: "aexp \<Rightarrow> 'av st \<Rightarrow> 'av" where
 "aval' (V x) S = fun S x" |
 "aval' (Plus a1 a2) S = plus' (aval' a1 S) (aval' a2 S)"
 
-lemma aval'_sound: "s : \<gamma>\<^isub>s S \<Longrightarrow> vars a \<subseteq> dom S \<Longrightarrow> aval a s : \<gamma>(aval' a S)"
+lemma aval'_sound: "s : \<gamma>\<^isub>s S \<Longrightarrow> aval a s : \<gamma>(aval' a S)"
 by (induction a) (auto simp: gamma_num' gamma_plus' \<gamma>_st_def)
 
 lemma gamma_Step_subcomm: fixes C1 C2 :: "'a::semilattice_sup acom"
-  assumes "!!x e S. x : X \<Longrightarrow> vars e \<subseteq> X \<Longrightarrow> S \<in> L X \<Longrightarrow> f1 x e (\<gamma>\<^isub>o S) \<subseteq> \<gamma>\<^isub>o (f2 x e S)"
-          "!!b S. S \<in> L X \<Longrightarrow> vars b \<subseteq> X \<Longrightarrow> g1 b (\<gamma>\<^isub>o S) \<subseteq> \<gamma>\<^isub>o (g2 b S)"
-  shows "C \<in> L X \<Longrightarrow> S \<in> L X \<Longrightarrow> Step f1 g1 (\<gamma>\<^isub>o S) (\<gamma>\<^isub>c C) \<le> \<gamma>\<^isub>c (Step f2 g2 S C)"
+  assumes "!!x e S. f1 x e (\<gamma>\<^isub>o S) \<subseteq> \<gamma>\<^isub>o (f2 x e S)"
+          "!!b S. g1 b (\<gamma>\<^isub>o S) \<subseteq> \<gamma>\<^isub>o (g2 b S)"
+  shows "Step f1 g1 (\<gamma>\<^isub>o S) (\<gamma>\<^isub>c C) \<le> \<gamma>\<^isub>c (Step f2 g2 S C)"
 proof(induction C arbitrary: S)
-qed (auto simp: assms intro!: mono_gamma_o post_in_L sup_ge1 sup_ge2)
+qed (auto simp: assms intro!: mono_gamma_o sup_ge1 sup_ge2)
 
 lemma in_gamma_update: "\<lbrakk> s : \<gamma>\<^isub>s S; i : \<gamma> a \<rbrakk> \<Longrightarrow> s(x := i) : \<gamma>\<^isub>s(update S x a)"
 by(simp add: \<gamma>_st_def)
 
 end
-
-
-lemma Step_in_L: fixes C :: "'a::semilatticeL acom"
-assumes "!!x e S. \<lbrakk>S \<in> L X; x \<in> X; vars e \<subseteq> X\<rbrakk> \<Longrightarrow> f x e S \<in> L X"
-        "!!b S. S \<in> L X \<Longrightarrow> vars b \<subseteq> X \<Longrightarrow> g b S \<in> L X"
-shows"\<lbrakk> C \<in> L X; S \<in> L X \<rbrakk> \<Longrightarrow> Step f g S C \<in> L X"
-proof(induction C arbitrary: S)
-  case Assign thus ?case
-    by(auto simp: L_st_def assms split: option.splits)
-qed (auto simp: assms)
 
 
 text{* The for-clause (here and elsewhere) only serves the purpose of fixing
@@ -85,7 +71,7 @@ definition "step' = Step
   (\<lambda>b S. S)"
 
 definition AI :: "com \<Rightarrow> 'av st option acom option" where
-"AI c = pfp (step' (Top(vars c))) (bot c)"
+"AI c = pfp (step' \<top>) (bot c)"
 
 
 lemma strip_step'[simp]: "strip(step' S C) = strip C"
@@ -94,32 +80,23 @@ by(simp add: step'_def)
 
 text{* Soundness: *}
 
-lemma step_step': "C \<in> L X \<Longrightarrow> S \<in> L X \<Longrightarrow> step (\<gamma>\<^isub>o S) (\<gamma>\<^isub>c C) \<le> \<gamma>\<^isub>c (step' S C)"
+lemma step_step': "step (\<gamma>\<^isub>o S) (\<gamma>\<^isub>c C) \<le> \<gamma>\<^isub>c (step' S C)"
 unfolding step_def step'_def
 by(rule gamma_Step_subcomm)
-  (auto simp: L_st_def intro!: aval'_sound in_gamma_update split: option.splits)
-
-lemma step'_in_L[simp]: "\<lbrakk> C \<in> L X; S \<in> L X \<rbrakk> \<Longrightarrow> step' S C \<in> L X"
-unfolding step'_def
-by(rule Step_in_L)(auto simp: L_st_def step'_def split: option.splits)
+  (auto simp: intro!: aval'_sound in_gamma_update split: option.splits)
 
 lemma AI_sound: "AI c = Some C \<Longrightarrow> CS c \<le> \<gamma>\<^isub>c C"
 proof(simp add: CS_def AI_def)
-  assume 1: "pfp (step' (Top(vars c))) (bot c) = Some C"
-  have "C \<in> L(vars c)"
-    by(rule pfp_inv[where P = "%C. C \<in> L(vars c)", OF 1 _ bot_in_L])
-      (erule step'_in_L[OF _ Top_in_L])
-  have pfp': "step' (Top(vars c)) C \<le> C" by(rule pfp_pfp[OF 1])
-  have 2: "step (\<gamma>\<^isub>o(Top(vars c))) (\<gamma>\<^isub>c C) \<le> \<gamma>\<^isub>c C"
+  assume 1: "pfp (step' \<top>) (bot c) = Some C"
+  have pfp': "step' \<top> C \<le> C" by(rule pfp_pfp[OF 1])
+  have 2: "step (\<gamma>\<^isub>o \<top>) (\<gamma>\<^isub>c C) \<le> \<gamma>\<^isub>c C"  --"transfer the pfp'"
   proof(rule order_trans)
-    show "step (\<gamma>\<^isub>o (Top(vars c))) (\<gamma>\<^isub>c C) \<le>  \<gamma>\<^isub>c (step' (Top(vars c)) C)"
-      by(rule step_step'[OF `C \<in> L(vars c)` Top_in_L])
-    show "\<gamma>\<^isub>c (step' (Top(vars c)) C) \<le> \<gamma>\<^isub>c C"
-      by(rule mono_gamma_c[OF pfp'])
+    show "step (\<gamma>\<^isub>o \<top>) (\<gamma>\<^isub>c C) \<le> \<gamma>\<^isub>c (step' \<top> C)" by(rule step_step')
+    show "... \<le> \<gamma>\<^isub>c C" by (metis mono_gamma_c[OF pfp'])
   qed
   have 3: "strip (\<gamma>\<^isub>c C) = c" by(simp add: strip_pfp[OF _ 1] step'_def)
-  have "lfp c (step (\<gamma>\<^isub>o(Top(vars c)))) \<le> \<gamma>\<^isub>c C"
-    by(rule lfp_lowerbound[simplified,where f="step (\<gamma>\<^isub>o(Top(vars c)))", OF 3 2])
+  have "lfp c (step (\<gamma>\<^isub>o \<top>)) \<le> \<gamma>\<^isub>c C"
+    by(rule lfp_lowerbound[simplified,where f="step (\<gamma>\<^isub>o \<top>)", OF 3 2])
   thus "lfp c (step UNIV) \<le> \<gamma>\<^isub>c C" by simp
 qed
 
@@ -128,49 +105,34 @@ end
 
 subsubsection "Monotonicity"
 
-lemma le_sup_disj: "y \<in> L X \<Longrightarrow> (z::_::semilatticeL) \<in> L X \<Longrightarrow>
-  x \<le> y \<or> x \<le> z \<Longrightarrow> x \<le> y \<squnion> z"
+lemma le_sup_disj: "x \<le> y \<or> x \<le> z \<Longrightarrow> x \<le> y \<squnion> (z::_::semilattice_sup)"
 by (metis sup_ge1 sup_ge2 order_trans)
 
-theorem mono2_Step: fixes C1 :: "'a::semilatticeL acom"
-  assumes "!!x e S1 S2. \<lbrakk>S1 \<in> L X; S2 \<in> L X; x \<in> X; vars e \<subseteq> X; S1 \<le> S2\<rbrakk> \<Longrightarrow> f x e S1 \<le> f x e S2"
-          "!!b S1 S2. S1 \<in> L X \<Longrightarrow> S2 \<in> L X \<Longrightarrow> vars b \<subseteq> X \<Longrightarrow> S1 \<le> S2 \<Longrightarrow> g b S1 \<le> g b S2"
-  shows "S1 \<in> L X \<Longrightarrow> S2 \<in> L X \<Longrightarrow> C1 \<in> L X \<Longrightarrow> C2 \<in> L X \<Longrightarrow>
-  S1 \<le> S2 \<Longrightarrow> C1 \<le> C2 \<Longrightarrow> Step f g S1 C1 \<le> Step f g S2 C2"
+theorem mono2_Step: fixes C1 :: "'a::semilattice acom"
+  assumes "!!x e S1 S2. S1 \<le> S2 \<Longrightarrow> f x e S1 \<le> f x e S2"
+          "!!b S1 S2. S1 \<le> S2 \<Longrightarrow> g b S1 \<le> g b S2"
+  shows "S1 \<le> S2 \<Longrightarrow> C1 \<le> C2 \<Longrightarrow> Step f g S1 C1 \<le> Step f g S2 C2"
 by(induction C1 C2 arbitrary: S1 S2 rule: less_eq_acom.induct)
-  (auto simp: mono_post assms le_sup_disj le_sup_disj[OF  post_in_L post_in_L])
+  (auto simp: mono_post assms le_sup_disj)
 
 
 locale Abs_Int_mono = Abs_Int +
 assumes mono_plus': "a1 \<le> b1 \<Longrightarrow> a2 \<le> b2 \<Longrightarrow> plus' a1 a2 \<le> plus' b1 b2"
 begin
 
-lemma mono_aval':
-  "S1 \<le> S2 \<Longrightarrow> S1 \<in> L X \<Longrightarrow> S2 \<in> L X \<Longrightarrow> vars e \<subseteq> X \<Longrightarrow> aval' e S1 \<le> aval' e S2"
-by(induction e) (auto simp: less_eq_st_def mono_plus' L_st_def)
+lemma mono_aval': "S1 \<le> S2 \<Longrightarrow> aval' e S1 \<le> aval' e S2"
+by(induction e) (auto simp: mono_plus' mono_fun)
 
-theorem mono_step': "S1 \<in> L X \<Longrightarrow> S2 \<in> L X \<Longrightarrow> C1 \<in> L X \<Longrightarrow> C2 \<in> L X \<Longrightarrow>
-  S1 \<le> S2 \<Longrightarrow> C1 \<le> C2 \<Longrightarrow> step' S1 C1 \<le> step' S2 C2"
+theorem mono_step': "S1 \<le> S2 \<Longrightarrow> C1 \<le> C2 \<Longrightarrow> step' S1 C1 \<le> step' S2 C2"
 unfolding step'_def
 by(rule mono2_Step) (auto simp: mono_aval' split: option.split)
 
-lemma mono_step'_top: "C \<in> L X \<Longrightarrow> C' \<in> L X \<Longrightarrow>
-  C \<le> C' \<Longrightarrow> step' (Top X) C \<le> step' (Top X) C'"
-by (metis Top_in_L mono_step' order_refl)
+lemma mono_step'_top: "C \<le> C' \<Longrightarrow> step' \<top> C \<le> step' \<top> C'"
+by (metis mono_step' order_refl)
 
-lemma pfp_bot_least:
-assumes "\<forall>x\<in>L(vars c)\<inter>{C. strip C = c}.\<forall>y\<in>L(vars c)\<inter>{C. strip C = c}.
-  x \<le> y \<longrightarrow> f x \<le> f y"
-and "\<forall>C. C \<in> L(vars c)\<inter>{C. strip C = c} \<longrightarrow> f C \<in> L(vars c)\<inter>{C. strip C = c}"
-and "f C' \<le> C'" "strip C' = c" "C' \<in> L(vars c)" "pfp f (bot c) = Some C"
+lemma AI_least_pfp: assumes "AI c = Some C" "step' \<top> C' \<le> C'" "strip C' = c"
 shows "C \<le> C'"
-by(rule while_least[OF assms(1,2) _ _ assms(3) _ assms(6)[unfolded pfp_def]])
-  (simp_all add: assms(4,5) bot_least)
-
-lemma AI_least_pfp: assumes "AI c = Some C"
-and "step' (Top(vars c)) C' \<le> C'" "strip C' = c" "C' \<in> L(vars c)"
-shows "C \<le> C'"
-by(rule pfp_bot_least[OF _ _ assms(2-4) assms(1)[unfolded AI_def]])
+by(rule pfp_bot_least[OF _ _ assms(2,3) assms(1)[unfolded AI_def]])
   (simp_all add: mono_step'_top)
 
 end
@@ -196,43 +158,111 @@ qed
 
 
 locale Measure1 =
-fixes m :: "'av::order \<Rightarrow> nat"
+fixes m :: "'av::{order,top} \<Rightarrow> nat"
 fixes h :: "nat"
 assumes h: "m x \<le> h"
 begin
 
-definition m_s :: "'av st \<Rightarrow> nat" ("m\<^isub>s") where
-"m_s S = (\<Sum> x \<in> dom S. m(fun S x))"
+definition m_s :: "vname set \<Rightarrow> 'av st \<Rightarrow> nat" ("m\<^isub>s") where
+"m_s X S = (\<Sum> x \<in> X. m(fun S x))"
 
-lemma m_s_h: "x \<in> L X \<Longrightarrow> finite X \<Longrightarrow> m_s x \<le> h * card X"
-by(simp add: L_st_def m_s_def)
-  (metis nat_mult_commute of_nat_id setsum_bounded[OF h])
+lemma m_s_h: "finite X \<Longrightarrow> m_s X S \<le> h * card X"
+by(simp add: m_s_def) (metis nat_mult_commute of_nat_id setsum_bounded[OF h])
 
-definition m_o :: "nat \<Rightarrow> 'av st option \<Rightarrow> nat" ("m\<^isub>o") where
-"m_o d opt = (case opt of None \<Rightarrow> h*d+1 | Some S \<Rightarrow> m_s S)"
+definition m_o :: "vname set \<Rightarrow> 'av st option \<Rightarrow> nat" ("m\<^isub>o") where
+"m_o X opt = (case opt of None \<Rightarrow> h * card X + 1 | Some S \<Rightarrow> m_s X S)"
 
-lemma m_o_h: "ost \<in> L X \<Longrightarrow> finite X \<Longrightarrow> m_o (card X) ost \<le> (h*card X + 1)"
-by(auto simp add: m_o_def m_s_h split: option.split dest!:m_s_h)
+lemma m_o_h: "finite X \<Longrightarrow> m_o X opt \<le> (h*card X + 1)"
+by(auto simp add: m_o_def m_s_h le_SucI split: option.split dest:m_s_h)
 
 definition m_c :: "'av st option acom \<Rightarrow> nat" ("m\<^isub>c") where
-"m_c C = (\<Sum>i<size(annos C). m_o (card(vars(strip C))) (annos C ! i))"
+"m_c C = (\<Sum>i<size(annos C). m_o (vars C) (annos C ! i))"
 
-lemma m_c_h: assumes "C \<in> L(vars(strip C))"
-shows "m_c C \<le> size(annos C) * (h * card(vars(strip C)) + 1)"
+text{* Upper complexity bound: *}
+lemma m_c_h: "m_c C \<le> size(annos C) * (h * card(vars C) + 1)"
 proof-
-  let ?X = "vars(strip C)" let ?n = "card ?X" let ?a = "size(annos C)"
-  { fix i assume "i < ?a"
-    hence "annos C ! i \<in> L ?X" using assms by(simp add: L_acom_def)
-    note m_o_h[OF this finite_cvars]
-  } note 1 = this
-  have "m_c C = (\<Sum>i<?a. m_o ?n (annos C ! i))" by(simp add: m_c_def)
+  let ?X = "vars C" let ?n = "card ?X" let ?a = "size(annos C)"
+  have "m_c C = (\<Sum>i<?a. m_o ?X (annos C ! i))" by(simp add: m_c_def)
   also have "\<dots> \<le> (\<Sum>i<?a. h * ?n + 1)"
-    apply(rule setsum_mono) using 1 by simp
+    apply(rule setsum_mono) using m_o_h[OF finite_Cvars] by simp
   also have "\<dots> = ?a * (h * ?n + 1)" by simp
   finally show ?thesis .
 qed
 
 end
+
+text{* The predicates @{text "top_on X a"} that follow describe that @{text a} is some object
+that maps all variables in @{text X} to @{term \<top>}.
+This is an important invariant for the termination proof where we argue that only
+the finitely many variables in the program change. That the others do not change
+follows because they remain @{term \<top>}. *}
+
+class top_on =
+fixes top_on :: "vname set \<Rightarrow> 'a \<Rightarrow> bool"
+
+instantiation st :: (top)top_on
+begin
+
+fun top_on_st :: "vname set \<Rightarrow> 'a st \<Rightarrow> bool" where
+"top_on_st X F = (\<forall>x\<in>X. fun F x = \<top>)"
+
+instance ..
+
+end
+
+instantiation option :: (top_on)top_on
+begin
+
+fun top_on_option :: "vname set \<Rightarrow> 'a option \<Rightarrow> bool" where
+"top_on_option X (Some F) = top_on X F" |
+"top_on_option X None = True"
+
+instance ..
+
+end
+
+instantiation acom :: (top_on)top_on
+begin
+
+definition top_on_acom :: "vname set \<Rightarrow> 'a acom \<Rightarrow> bool" where
+"top_on_acom X C = (\<forall>a \<in> set(annos C). top_on X a)"
+
+instance ..
+
+end
+
+lemma top_on_top: "top_on X (\<top>::_ st option)"
+by(auto simp: top_option_def fun_top)
+
+lemma top_on_bot: "top_on X (bot c)"
+by(auto simp add: top_on_acom_def bot_def)
+
+lemma top_on_post: "top_on X C \<Longrightarrow> top_on X (post C)"
+by(simp add: top_on_acom_def post_in_annos)
+
+lemma top_on_acom_simps:
+  "top_on X (SKIP {Q}) = top_on X Q"
+  "top_on X (x ::= e {Q}) = top_on X Q"
+  "top_on X (C1;C2) = (top_on X C1 \<and> top_on X C2)"
+  "top_on X (IF b THEN {P1} C1 ELSE {P2} C2 {Q}) =
+   (top_on X P1 \<and> top_on X C1 \<and> top_on X P2 \<and> top_on X C2 \<and> top_on X Q)"
+  "top_on X ({I} WHILE b DO {P} C {Q}) =
+   (top_on X I \<and> top_on X C \<and> top_on X P \<and> top_on X Q)"
+by(auto simp add: top_on_acom_def)
+
+lemma top_on_sup:
+  "top_on X o1 \<Longrightarrow> top_on X o2 \<Longrightarrow> top_on X (o1 \<squnion> o2 :: _ st option)"
+apply(induction o1 o2 rule: sup_option.induct)
+apply(auto)
+by transfer simp
+
+lemma top_on_Step: fixes C :: "('a::semilattice)st option acom"
+assumes "!!x e S. \<lbrakk>top_on X S; x \<notin> X; vars e \<subseteq> -X\<rbrakk> \<Longrightarrow> top_on X (f x e S)"
+        "!!b S. top_on X S \<Longrightarrow> vars b \<subseteq> -X \<Longrightarrow> top_on X (g b S)"
+shows "\<lbrakk> vars C \<subseteq> -X; top_on X S; top_on X C \<rbrakk> \<Longrightarrow> top_on X (Step f g S C)"
+proof(induction C arbitrary: S)
+qed (auto simp: top_on_acom_simps vars_acom_def top_on_post top_on_sup assms)
+
 
 locale Measure = Measure1 +
 assumes m2: "x < y \<Longrightarrow> m x > m y"
@@ -241,62 +271,79 @@ begin
 lemma m1: "x \<le> y \<Longrightarrow> m x \<ge> m y"
 by(auto simp: le_less m2)
 
-lemma m_s2: "finite(dom S1) \<Longrightarrow> S1 < S2 \<Longrightarrow> m_s S1 > m_s S2"
-proof(auto simp add: less_st_def less_eq_st_def m_s_def)
-  assume "finite(dom S2)" and 0: "\<forall>x\<in>dom S2. fun S1 x \<le> fun S2 x"
-  hence 1: "\<forall>x\<in>dom S2. m(fun S1 x) \<ge> m(fun S2 x)" by (metis m1)
-  fix x assume "x \<in> dom S2" "\<not> fun S2 x \<le> fun S1 x"
-  hence 2: "\<exists>x\<in>dom S2. m(fun S1 x) > m(fun S2 x)" by (metis 0 m2 less_le_not_le)
-  from setsum_strict_mono_ex1[OF `finite(dom S2)` 1 2]
-  show "(\<Sum>x\<in>dom S2. m (fun S2 x)) < (\<Sum>x\<in>dom S2. m (fun S1 x))" .
+lemma m_s2_rep: assumes "finite(X)" and "S1 = S2 on -X" and "\<forall>x. S1 x \<le> S2 x" and "S1 \<noteq> S2"
+shows "(\<Sum>x\<in>X. m (S2 x)) < (\<Sum>x\<in>X. m (S1 x))"
+proof-
+  from assms(3) have 1: "\<forall>x\<in>X. m(S1 x) \<ge> m(S2 x)" by (simp add: m1)
+  from assms(2,3,4) have "EX x:X. S1 x < S2 x"
+    by(simp add: fun_eq_iff) (metis Compl_iff le_neq_trans)
+  hence 2: "\<exists>x\<in>X. m(S1 x) > m(S2 x)" by (metis m2)
+  from setsum_strict_mono_ex1[OF `finite X` 1 2]
+  show "(\<Sum>x\<in>X. m (S2 x)) < (\<Sum>x\<in>X. m (S1 x))" .
 qed
 
-lemma m_o2: "finite X \<Longrightarrow> o1 \<in> L X \<Longrightarrow> o2 \<in> L X \<Longrightarrow>
-  o1 < o2 \<Longrightarrow> m_o (card X) o1 > m_o (card X) o2"
+lemma m_s2: "finite(X) \<Longrightarrow> fun S1 = fun S2 on -X \<Longrightarrow> S1 < S2 \<Longrightarrow> m_s X S1 > m_s X S2"
+apply(auto simp add: less_st_def m_s_def)
+apply (transfer fixing: m)
+apply(simp add: less_eq_st_rep_iff eq_st_def m_s2_rep)
+done
+
+lemma m_o2: "finite X \<Longrightarrow> top_on (-X) o1 \<Longrightarrow> top_on (-X) o2 \<Longrightarrow>
+  o1 < o2 \<Longrightarrow> m_o X o1 > m_o X o2"
 proof(induction o1 o2 rule: less_eq_option.induct)
-  case 1 thus ?case by (auto simp: m_o_def L_st_def m_s2 less_option_def)
+  case 1 thus ?case by (auto simp: m_o_def m_s2 less_option_def)
 next
   case 2 thus ?case by(auto simp: m_o_def less_option_def le_imp_less_Suc m_s_h)
 next
   case 3 thus ?case by (auto simp: less_option_def)
 qed
 
-lemma m_o1: "finite X \<Longrightarrow> o1 \<in> L X \<Longrightarrow> o2 \<in> L X \<Longrightarrow>
-  o1 \<le> o2 \<Longrightarrow> m_o (card X) o1 \<ge> m_o (card X) o2"
+lemma m_o1: "finite X \<Longrightarrow> top_on (-X) o1 \<Longrightarrow> top_on (-X) o2 \<Longrightarrow>
+  o1 \<le> o2 \<Longrightarrow> m_o X o1 \<ge> m_o X o2"
 by(auto simp: le_less m_o2)
 
-lemma m_c2: "C1 \<in> L(vars(strip C1)) \<Longrightarrow> C2 \<in> L(vars(strip C2)) \<Longrightarrow>
+
+lemma m_c2: "top_on (-vars C1) C1 \<Longrightarrow> top_on (-vars C2) C2 \<Longrightarrow>
   C1 < C2 \<Longrightarrow> m_c C1 > m_c C2"
-proof(auto simp add: le_iff_le_annos m_c_def size_annos_same[of C1 C2] less_acom_def L_acom_def)
+proof(auto simp add: le_iff_le_annos m_c_def size_annos_same[of C1 C2] vars_acom_def less_acom_def)
   let ?X = "vars(strip C2)"
-  let ?n = "card ?X"
-  assume V1: "\<forall>a\<in>set(annos C1). a \<in> L ?X"
-    and V2: "\<forall>a\<in>set(annos C2). a \<in> L ?X"
-    and strip_eq: "strip C1 = strip C2"
-    and 0: "\<forall>i<size(annos C2). annos C1 ! i \<le> annos C2 ! i"
-  hence 1: "\<forall>i<size(annos C2). m_o ?n (annos C1 ! i) \<ge> m_o ?n (annos C2 ! i)"
-    by (auto simp: all_set_conv_all_nth)
-       (metis finite_cvars m_o1 size_annos_same2)
-  fix i assume "i < size(annos C2)" "\<not> annos C2 ! i \<le> annos C1 ! i"
-  hence "m_o ?n (annos C1 ! i) > m_o ?n (annos C2 ! i)" (is "?P i")
-    by(metis m_o2[OF finite_cvars] V1 V2 nth_mem size_annos_same[OF strip_eq] 0 less_option_def)
+  assume top: "top_on (- vars(strip C2)) C1"  "top_on (- vars(strip C2)) C2"
+  and strip_eq: "strip C1 = strip C2"
+  and 0: "\<forall>i<size(annos C2). annos C1 ! i \<le> annos C2 ! i"
+  hence 1: "\<forall>i<size(annos C2). m_o ?X (annos C1 ! i) \<ge> m_o ?X (annos C2 ! i)"
+    apply (auto simp: all_set_conv_all_nth vars_acom_def top_on_acom_def)
+    by (metis finite_cvars m_o1 size_annos_same2)
+  fix i assume i: "i < size(annos C2)" "\<not> annos C2 ! i \<le> annos C1 ! i"
+  have topo1: "top_on (- ?X) (annos C1 ! i)"
+    using i(1) top(1) by(simp add: top_on_acom_def size_annos_same[OF strip_eq])
+  have topo2: "top_on (- ?X) (annos C2 ! i)"
+    using i(1) top(2) by(simp add: top_on_acom_def size_annos_same[OF strip_eq])
+  from i have "m_o ?X (annos C1 ! i) > m_o ?X (annos C2 ! i)" (is "?P i")
+    by (metis 0 less_option_def m_o2[OF finite_cvars topo1] topo2)
   hence 2: "\<exists>i < size(annos C2). ?P i" using `i < size(annos C2)` by blast
-  show "(\<Sum>i<size(annos C2). m_o ?n (annos C2 ! i))
-         < (\<Sum>i<size(annos C2). m_o ?n (annos C1 ! i))"
+  show "(\<Sum>i<size(annos C2). m_o ?X (annos C2 ! i))
+         < (\<Sum>i<size(annos C2). m_o ?X (annos C1 ! i))"
     apply(rule setsum_strict_mono_ex1) using 1 2 by (auto)
 qed
 
 end
+
 
 locale Abs_Int_measure =
   Abs_Int_mono where \<gamma>=\<gamma> + Measure where m=m
   for \<gamma> :: "'av::semilattice \<Rightarrow> val set" and m :: "'av \<Rightarrow> nat"
 begin
 
+lemma top_on_step': "\<lbrakk> vars C \<subseteq> -X; top_on X C \<rbrakk> \<Longrightarrow> top_on X (step' \<top> C)"
+unfolding step'_def
+by(rule top_on_Step)
+  (auto simp add: top_option_def fun_top split: option.splits)
+
 lemma AI_Some_measure: "\<exists>C. AI c = Some C"
 unfolding AI_def
-apply(rule pfp_termination[where I = "\<lambda>C. strip C = c \<and> C \<in> L(vars c)" and m="m_c"])
-apply(simp_all add: m_c2 mono_step'_top bot_least)
+apply(rule pfp_termination[where I = "\<lambda>C. strip C = c \<and> top_on (- vars C) C" and m="m_c"])
+apply(simp_all add: m_c2 mono_step'_top bot_least top_on_bot)
+apply(auto simp add: top_on_step' vars_acom_def)
 done
 
 end
