src/HOL/IMP/Abs_State.thy
@@ -4,133 +4,56 @@ theory Abs_State
 imports Abs_Int0
 begin
 
-subsubsection "Set-based lattices"
+type_synonym 'a st_rep = "(vname * 'a) list"
 
+definition fun_rep :: "('a::top) st_rep \<Rightarrow> vname \<Rightarrow> 'a" where
+"fun_rep ps = (\<lambda>x. case map_of ps x of Some a \<Rightarrow> a | None \<Rightarrow> \<top>)"
 
-class L =
-fixes L :: "vname set \<Rightarrow> 'a set"
+definition eq_st :: "('a::top) st_rep \<Rightarrow> 'a st_rep \<Rightarrow> bool" where
+"eq_st S1 S2 = (fun_rep S1 = fun_rep S2)"
 
+quotient_type 'a st = "('a::top) st_rep" / eq_st
+by (metis eq_st_def equivpI reflpI sympI transpI)
 
-instantiation acom :: (L)L
-begin
+lemma st_cons[simp]: "fun_rep ((x,y) # ps) = (fun_rep ps) (x := y)"
+by(auto simp: fun_rep_def fun_eq_iff split: option.splits if_splits)
 
-definition L_acom where
-"L X = {C. vars(strip C) \<subseteq> X \<and> (\<forall>a \<in> set(annos C). a \<in> L X)}"
+lift_definition update :: "('a::top) st \<Rightarrow> vname \<Rightarrow> 'a \<Rightarrow> 'a st" is "\<lambda>ps x a. (x,a)#ps"
+by(auto simp: eq_st_def)
 
-instance ..
+lift_definition "fun" :: "('a::top) st \<Rightarrow> vname \<Rightarrow> 'a" is fun_rep
+by(simp add: eq_st_def)
 
-end
+definition show_st :: "vname set \<Rightarrow> ('a::top) st \<Rightarrow> (vname * 'a)set" where
+"show_st X S = (\<lambda>x. (x, fun S x)) ` X"
 
-
-instantiation option :: (L)L
-begin
-
-definition L_option where
-"L X = {opt. case opt of None \<Rightarrow> True | Some x \<Rightarrow> x \<in> L X}"
-
-lemma L_option_simps[simp]: "None \<in> L X" "(Some x \<in> L X) = (x \<in> L X)"
-by(simp_all add: L_option_def)
-
-instance ..
-
-end
-
-class semilatticeL = order + sup + L +
-fixes Top :: "vname set \<Rightarrow> 'a"
-assumes sup_ge1 [simp]: "x \<in> L X \<Longrightarrow> y \<in> L X \<Longrightarrow> x \<le> x \<squnion> y"
-and sup_ge2 [simp]: "x \<in> L X \<Longrightarrow> y \<in> L X \<Longrightarrow> y \<le> x \<squnion> y"
-and sup_least[simp]: "x \<le> z \<Longrightarrow> y \<le> z \<Longrightarrow> x \<squnion> y \<le> z"
-and Top[simp]: "x \<in> L X \<Longrightarrow> x \<le> Top X"
-and Top_in_L[simp]: "Top X \<in> L X"
-and sup_in_L[simp]: "x \<in> L X \<Longrightarrow> y \<in> L X \<Longrightarrow> x \<squnion> y \<in> L X"
-
-notation (input) Top ("\<top>\<^bsub>_\<^esub>")
-notation (latex output) Top ("\<top>\<^bsub>\<^raw:\isa{>_\<^raw:}>\<^esub>")
-
-instantiation option :: (semilatticeL)semilatticeL
-begin
-
-definition Top_option where "Top c = Some(Top c)"
-
-instance proof
-  case goal1 thus ?case by(cases x, simp, cases y, simp_all)
-next
-  case goal2 thus ?case by(cases y, simp, cases x, simp_all)
-next
-  case goal3 thus ?case by(cases z, simp, cases y, simp, cases x, simp_all)
-next
-  case goal4 thus ?case by(cases x, simp_all add: Top_option_def)
-next
-  case goal5 thus ?case by(simp add: Top_option_def)
-next
-  case goal6 thus ?case by(simp add: L_option_def split: option.splits)
-qed
-
-end
-
-
-subsection "Abstract State with Computable Ordering"
-
-hide_type  st  --"to avoid long names"
-
-text{* A concrete type of state with computable @{text"\<le>"}: *}
-
-fun st :: "(vname \<Rightarrow> 'a) * vname set \<Rightarrow> bool" where
-"st (f,X) = (\<forall>x. x \<notin> X \<longrightarrow> f x = undefined)"
-
-typedef 'a st = "{p :: (vname \<Rightarrow> 'a) * vname set. st p}"
-proof
-  show "(\<lambda>x. undefined,{}) \<in> {p. st p}" by simp
-qed
-
-setup_lifting type_definition_st
-
-lift_definition St :: "(vname \<Rightarrow> 'a) \<Rightarrow> vname set \<Rightarrow> 'a st" is
-  "\<lambda>f X. (\<lambda>x. if x \<in> X then f x else undefined, X)"
-by(simp)
-
-lift_definition update :: "'a st \<Rightarrow> vname \<Rightarrow> 'a \<Rightarrow> 'a st" is
-  "\<lambda>(f,X) x a. (f(x := a), insert x X)"
-by(auto)
-
-lift_definition "fun" :: "'a st \<Rightarrow> vname \<Rightarrow> 'a" is fst ..
-
-lift_definition dom :: "'a st \<Rightarrow> vname set" is snd ..
-
-lemma dom_St[simp]: "dom(St f X) = X"
-by(simp add: St.rep_eq dom.rep_eq)
-
-lemma fun_St[simp]: "fun(St f X) = (\<lambda>x. if x \<in> X then f x else undefined)"
-by(simp add: St.rep_eq fun.rep_eq)
-
-definition show_st :: "'a st \<Rightarrow> (vname * 'a)set" where
-"show_st S = (\<lambda>x. (x, fun S x)) ` dom S"
-
-definition "show_acom = map_acom (Option.map show_st)"
+definition "show_acom C = map_acom (Option.map (show_st (vars(strip C)))) C"
 definition "show_acom_opt = Option.map show_acom"
 
 lemma fun_update[simp]: "fun (update S x y) = (fun S)(x:=y)"
 by transfer auto
 
-lemma dom_update[simp]: "dom (update S x y) = insert x (dom S)"
-by transfer auto
+definition \<gamma>_st :: "(('a::top) \<Rightarrow> 'b set) \<Rightarrow> 'a st \<Rightarrow> (vname \<Rightarrow> 'b) set" where
+"\<gamma>_st \<gamma> F = {f. \<forall>x. f x \<in> \<gamma>(fun F x)}"
 
-definition \<gamma>_st :: "('a \<Rightarrow> 'b set) \<Rightarrow> 'a st \<Rightarrow> (vname \<Rightarrow> 'b) set" where
-"\<gamma>_st \<gamma> F = {f. \<forall>x\<in>dom  F. f x \<in> \<gamma>(fun F x)}"
-
-lemma ext_st: "dom F = dom G \<Longrightarrow> \<forall>x \<in> dom G. fun F x = fun G x \<Longrightarrow> F=G"
-apply(induct F rule:Abs_st_induct)
-apply(induct G rule:Abs_st_induct)
-apply (auto simp:Abs_st_inject fun_def dom_def Abs_st_inverse simp del: st.simps)
-apply(rule ext)
-apply auto
-done
-
-instantiation st :: (order) order
+instantiation st :: ("{order,top}") order
 begin
 
-definition less_eq_st :: "'a st \<Rightarrow> 'a st \<Rightarrow> bool" where
-"F \<le> (G::'a st) = (dom F = dom G \<and> (\<forall>x \<in> dom F. fun F x \<le> fun G x))"
+definition less_eq_st_rep :: "'a st_rep \<Rightarrow> 'a st_rep \<Rightarrow> bool" where
+"less_eq_st_rep ps1 ps2 =
+  ((\<forall>x \<in> set(map fst ps1) \<union> set(map fst ps2). fun_rep ps1 x \<le> fun_rep ps2 x))"
+
+lemma less_eq_st_rep_iff: "less_eq_st_rep r1 r2 = (\<forall>x. fun_rep r1 x \<le> fun_rep r2 x)"
+apply(auto simp: less_eq_st_rep_def fun_rep_def split: option.split)
+apply (metis Un_iff map_of_eq_None_iff option.distinct(1))
+apply (metis Un_iff map_of_eq_None_iff option.distinct(1))
+done
+
+corollary less_eq_st_rep_iff_fun: "less_eq_st_rep r1 r2 = (fun_rep r1 \<le> fun_rep r2)"
+by (metis less_eq_st_rep_iff le_fun_def)
+
+lift_definition less_eq_st :: "'a st \<Rightarrow> 'a st \<Rightarrow> bool" is less_eq_st_rep
+by(auto simp add: eq_st_def less_eq_st_rep_iff)
 
 definition less_st where "F < (G::'a st) = (F \<le> G \<and> \<not> G \<le> F)"
 
@@ -138,61 +61,64 @@ instance
 proof
   case goal1 show ?case by(rule less_st_def)
 next
-  case goal2 show ?case by(auto simp: less_eq_st_def)
+  case goal2 show ?case by transfer (auto simp: less_eq_st_rep_def)
 next
-  case goal3 thus ?case by(fastforce simp: less_eq_st_def)
+  case goal3 thus ?case
+    by transfer (metis less_eq_st_rep_iff order_trans)
 next
-  case goal4 thus ?case by (metis less_eq_st_def antisym ext_st)
+  case goal4 thus ?case
+    by transfer (metis less_eq_st_rep_iff eq_st_def fun_eq_iff antisym)
 qed
 
 end
 
-instantiation st :: (sup) sup
+lemma le_st_iff: "(F \<le> G) = (\<forall>x. fun F x \<le> fun G x)"
+by transfer (rule less_eq_st_rep_iff)
+
+fun map2_st_rep :: "('a::top \<Rightarrow> 'a \<Rightarrow> 'a) \<Rightarrow> 'a st_rep \<Rightarrow> 'a st_rep \<Rightarrow> 'a st_rep" where
+"map2_st_rep f [] ps2 = map (%(x,y). (x, f \<top> y)) ps2" |
+"map2_st_rep f ((x,y)#ps1) ps2 =
+  (let y2 = (case map_of ps2 x of Some y2 \<Rightarrow> y2 | None \<Rightarrow> \<top>)
+   in (x,f y y2) # map2_st_rep f ps1 ps2)"
+
+lemma fun_rep_map2_rep[simp]:
+  "f \<top> \<top> = \<top> \<Longrightarrow> fun_rep (map2_st_rep f ps1 ps2) = (\<lambda>x. f (fun_rep ps1 x) (fun_rep ps2 x))"
+apply(induction f ps1 ps2 rule: map2_st_rep.induct)
+apply(simp add: fun_rep_def map_of_map fun_eq_iff split: option.split)
+apply(fastforce simp: fun_rep_def fun_eq_iff split:option.splits)
+done
+
+instantiation st :: (semilattice) semilattice
 begin
 
-definition sup_st :: "'a st \<Rightarrow> 'a st \<Rightarrow> 'a st" where
-"F \<squnion> (G::'a st) = St (\<lambda>x. fun F x \<squnion> fun G x) (dom F)"
+lift_definition sup_st :: "'a st \<Rightarrow> 'a st \<Rightarrow> 'a st" is "map2_st_rep (op \<squnion>)"
+by (simp add: eq_st_def)
 
-instance ..
-
-end
-
-instantiation st :: (type) L
-begin
-
-definition L_st :: "vname set \<Rightarrow> 'a st set" where
-"L(X::vname set) = {F. dom F = X}"
-
-instance ..
-
-end
-
-instantiation st :: (semilattice) semilatticeL
-begin
-
-definition Top_st :: "vname set \<Rightarrow> 'a st" where "Top(X) = St (\<lambda>x. \<top>) X"
+lift_definition top_st :: "'a st" is "[]"
+by(simp add: eq_st_def)
 
 instance
-proof qed(auto simp add: less_eq_st_def sup_st_def Top_st_def L_st_def)
+proof
+  case goal1 show ?case by transfer (simp add:less_eq_st_rep_iff)
+next
+  case goal2 show ?case by transfer (simp add:less_eq_st_rep_iff)
+next
+  case goal3 thus ?case by transfer (simp add:less_eq_st_rep_iff)
+next
+  case goal4 show ?case by transfer (simp add:less_eq_st_rep_iff fun_rep_def)
+qed
 
 end
 
-
-text{* Trick to make code generator happy. *}
-lemma [code]: "L = (L :: _ \<Rightarrow> _ st set)"
-by(rule refl)
-(* L is not used in the code but is part of a type class that is used.
-   Hence the code generator wants to build a dictionary with L in it.
-   But L is not executable. This looping defn makes it look as if it were. *)
-
-
-lemma mono_fun: "F \<le> G \<Longrightarrow> x : dom F \<Longrightarrow> fun F x \<le> fun G x"
-by(auto simp: less_eq_st_def)
+lemma fun_top: "fun \<top> = (\<lambda>x. \<top>)"
+by transfer (simp add: fun_rep_def)
 
 lemma mono_update[simp]:
   "a1 \<le> a2 \<Longrightarrow> S1 \<le> S2 \<Longrightarrow> update S1 x a1 \<le> update S2 x a2"
-by(auto simp add: less_eq_st_def)
+by transfer (auto simp add: less_eq_st_rep_def)
 
+lemma mono_fun: "S1 \<le> S2 \<Longrightarrow> fun S1 x \<le> fun S2 x"
+by transfer (simp add: less_eq_st_rep_iff)
 
 locale Gamma = Val_abs where \<gamma>=\<gamma> for \<gamma> :: "'av::semilattice \<Rightarrow> val set"
 begin
@@ -206,15 +132,14 @@ where "\<gamma>\<^isub>o == \<gamma>_option \<gamma>\<^isub>s"
 abbreviation \<gamma>\<^isub>c :: "'av st option acom \<Rightarrow> state set acom"
 where "\<gamma>\<^isub>c == map_acom \<gamma>\<^isub>o"
 
-lemma gamma_s_Top[simp]: "\<gamma>\<^isub>s (Top X) = UNIV"
-by(auto simp: Top_st_def \<gamma>_st_def)
+lemma gamma_s_top[simp]: "\<gamma>\<^isub>s \<top> = UNIV"
+by(auto simp: \<gamma>_st_def fun_top)
 
-lemma gamma_o_Top[simp]: "\<gamma>\<^isub>o (Top X) = UNIV"
-by (simp add: Top_option_def)
+lemma gamma_o_Top[simp]: "\<gamma>\<^isub>o \<top> = UNIV"
+by (simp add: top_option_def)
 
 lemma mono_gamma_s: "f \<le> g \<Longrightarrow> \<gamma>\<^isub>s f \<subseteq> \<gamma>\<^isub>s g"
-apply(simp add:\<gamma>_st_def subset_iff less_eq_st_def split: if_splits)
-by (metis mono_gamma subsetD)
+by(simp add:\<gamma>_st_def le_st_iff subset_iff) (metis mono_gamma subsetD)
 
 lemma mono_gamma_o:
   "S1 \<le> S2 \<Longrightarrow> \<gamma>\<^isub>o S1 \<subseteq> \<gamma>\<^isub>o S2"
